iris/IregDirBit.v
@@ -95,7 +95,7 @@ Section IregDirBit.
     assert (Hkey : (16 * Z.of_nat (ireg_bi inum) + Z.of_nat (islot inum))%Z
                    = bv_unsigned inum) by (symmetry; apply ireg_key_split).
     iMod (inv_acc E iregN with "Hinv") as "[Hbody Hclose]"; [exact HE |].
-    iDestruct "Hbody" as (m) "(>Ha & Hblks)".
+    iDestruct "Hbody" as (m) "(>Ha & Hblks & >Hreg)".
     pose proof (ireg_bi_lt inum nib Hin) as Hbi.
     iDestruct (ireg_blks_acc_upd γi γfs inodestart m nib (ireg_bi inum) Hbi
                 with "Hblks") as "[Hblk Hback]".
@@ -119,8 +119,8 @@ Section IregDirBit.
                ltac:(lia)). }
     assert (Hins : <[islot inum := ds !!! islot inum]> ds = ds).
     { apply list_insert_id, list_lookup_lookup_total_lt. lia. }
-    iMod ("Hclose" with "[Ha Hfsb Harm Hla Hep Hslback Hback]") as "_".
-    { iNext. iExists m. iFrame "Ha".
+    iMod ("Hclose" with "[Ha Hreg Hfsb Harm Hla Hep Hslback Hback]") as "_".
+    { iNext. iExists m. iFrame "Ha Hreg".
       iApply ("Hback" $! m with "[%] [Hfsb Harm Hla Hep Hslback]"); [done |].
       iExists ds. iSplitR; [done |]. iSplitR; [done |].
       iSplitL "Hfsb"; [iExact "Hfsb" |].
@@ -156,7 +156,7 @@ Section IregDirBit.
     assert (Hkey : (16 * Z.of_nat (ireg_bi inum) + Z.of_nat (islot inum))%Z
                    = bv_unsigned inum) by (symmetry; apply ireg_key_split).
     iMod (inv_acc E iregN with "Hinv") as "[Hbody Hclose]"; [exact HE |].
-    iDestruct "Hbody" as (m) "(>Ha & Hblks)".
+    iDestruct "Hbody" as (m) "(>Ha & Hblks & >Hreg)".
     pose proof (ireg_bi_lt inum nib Hin) as Hbi.
     iDestruct (ireg_blks_acc_upd γi γfs inodestart m nib (ireg_bi inum) Hbi
                 with "Hblks") as "[Hblk Hback]".
@@ -180,8 +180,8 @@ Section IregDirBit.
                ltac:(lia)). }
     assert (Hins : <[islot inum := ds !!! islot inum]> ds = ds).
     { apply list_insert_id, list_lookup_lookup_total_lt. lia. }
-    iMod ("Hclose" with "[Ha Hfsb Harm Hla Hep Hslback Hback]") as "_".
-    { iNext. iExists m. iFrame "Ha".
+    iMod ("Hclose" with "[Ha Hreg Hfsb Harm Hla Hep Hslback Hback]") as "_".
+    { iNext. iExists m. iFrame "Ha Hreg".
       iApply ("Hback" $! m with "[%] [Hfsb Harm Hla Hep Hslback]"); [done |].
       iExists ds. iSplitR; [done |]. iSplitR; [done |].
       iSplitL "Hfsb"; [iExact "Hfsb" |].
@@ -220,7 +220,7 @@ Section IregDirBit.
     assert (Hkey : (16 * Z.of_nat (ireg_bi inum) + Z.of_nat (islot inum))%Z
                    = bv_unsigned inum) by (symmetry; apply ireg_key_split).
     iMod (inv_acc E iregN with "Hinv") as "[Hbody Hclose]"; [exact HE |].
-    iDestruct "Hbody" as (m) "(>Ha & Hblks)".
+    iDestruct "Hbody" as (m) "(>Ha & Hblks & >Hreg)".
     pose proof (ireg_bi_lt inum nib Hin) as Hbi.
     iDestruct (ireg_blks_acc_upd γi γfs inodestart m nib (ireg_bi inum) Hbi
                 with "Hblks") as "[Hblk Hback]".
@@ -245,8 +245,8 @@ Section IregDirBit.
       pose proof (Hwl0 Hc'). lia. }
     assert (Hins : <[islot inum := ds !!! islot inum]> ds = ds).
     { apply list_insert_id, list_lookup_lookup_total_lt. lia. }
-    iMod ("Hclose" with "[Ha Hfsb Harm Hla Hep Hslback Hback]") as "_".
-    { iNext. iExists m. iFrame "Ha".
+    iMod ("Hclose" with "[Ha Hreg Hfsb Harm Hla Hep Hslback Hback]") as "_".
+    { iNext. iExists m. iFrame "Ha Hreg".
       iApply ("Hback" $! m with "[%] [Hfsb Harm Hla Hep Hslback]"); [done |].
       iExists ds. iSplitR; [done |]. iSplitR; [done |].
       iSplitL "Hfsb"; [iExact "Hfsb" |].
