iris/IregLinkNz.v
@@ -85,7 +85,7 @@ Section IregLinkNz.
     assert (Hkey : (16 * Z.of_nat (ireg_bi inum) + Z.of_nat (islot inum))%Z
                    = bv_unsigned inum) by (symmetry; apply ireg_key_split).
     iMod (inv_acc E iregN with "Hinv") as "[Hbody Hclose]"; [exact HE |].
-    iDestruct "Hbody" as (m) "(>Ha & Hblks)".
+    iDestruct "Hbody" as (m) "(>Ha & Hblks & >Hreg)".
     pose proof (ireg_bi_lt inum nib Hin) as Hbi.
     iDestruct (ireg_blks_acc_upd γi γfs inodestart m nib (ireg_bi inum) Hbi
                 with "Hblks") as "[Hblk Hback]".
@@ -107,8 +107,8 @@ Section IregLinkNz.
       destruct Hlok as [Hle _]. lia. }
     assert (Hins : <[islot inum := ds !!! islot inum]> ds = ds).
     { apply list_insert_id, list_lookup_lookup_total_lt. lia. }
-    iMod ("Hclose" with "[Ha Hfsb Harm Hla Hep Hslback Hback]") as "_".
-    { iNext. iExists m. iFrame "Ha".
+    iMod ("Hclose" with "[Ha Hreg Hfsb Harm Hla Hep Hslback Hback]") as "_".
+    { iNext. iExists m. iFrame "Ha Hreg".
       iApply ("Hback" $! m with "[%] [Hfsb Harm Hla Hep Hslback]"); [done |].
       iExists ds. iSplitR; [done |]. iSplitR; [done |].
       iSplitL "Hfsb"; [iExact "Hfsb" |].
@@ -158,7 +158,7 @@ Section IregLinkNz.
     assert (Hkey : (16 * Z.of_nat (ireg_bi inum) + Z.of_nat (islot inum))%Z
                    = bv_unsigned inum) by (symmetry; apply ireg_key_split).
     iMod (inv_acc E iregN with "Hinv") as "[Hbody Hclose]"; [exact HE |].
-    iDestruct "Hbody" as (m) "(>Ha & Hblks)".
+    iDestruct "Hbody" as (m) "(>Ha & Hblks & >Hreg)".
     pose proof (ireg_bi_lt inum nib Hin) as Hbi.
     iDestruct (ireg_blks_acc_upd γi γfs inodestart m nib (ireg_bi inum) Hbi
                 with "Hblks") as "[Hblk Hback]".
@@ -195,7 +195,7 @@ Section IregLinkNz.
     assert (Hkey : (16 * Z.of_nat (ireg_bi inum) + Z.of_nat (islot inum))%Z
                    = bv_unsigned inum) by (symmetry; apply ireg_key_split).
     iMod (inv_acc E iregN with "Hinv") as "[Hbody Hclose]"; [exact HE |].
-    iDestruct "Hbody" as (m) "(>Ha & Hblks)".
+    iDestruct "Hbody" as (m) "(>Ha & Hblks & >Hreg)".
     pose proof (ireg_bi_lt inum nib Hin) as Hbi.
     iDestruct (ireg_blks_acc_upd γi γfs inodestart m nib (ireg_bi inum) Hbi
                 with "Hblks") as "[Hblk Hback]".
@@ -216,8 +216,8 @@ Section IregLinkNz.
       destruct Hlok as [Hle _]. lia. }
     assert (Hins : <[islot inum := ds !!! islot inum]> ds = ds).
     { apply list_insert_id, list_lookup_lookup_total_lt. lia. }
-    iMod ("Hclose" with "[Ha Hfsb Harm Hla Hep Hslback Hback]") as "_".
-    { iNext. iExists m. iFrame "Ha".
+    iMod ("Hclose" with "[Ha Hreg Hfsb Harm Hla Hep Hslback Hback]") as "_".
+    { iNext. iExists m. iFrame "Ha Hreg".
       iApply ("Hback" $! m with "[%] [Hfsb Harm Hla Hep Hslback]"); [done |].
       iExists ds. iSplitR; [done |]. iSplitR; [done |].
       iSplitL "Hfsb"; [iExact "Hfsb" |].
@@ -251,7 +251,7 @@ Section IregLinkNz.
     assert (Hkey : (16 * Z.of_nat (ireg_bi inum) + Z.of_nat (islot inum))%Z
                    = bv_unsigned inum) by (symmetry; apply ireg_key_split).
     iMod (inv_acc E iregN with "Hinv") as "[Hbody Hclose]"; [exact HE |].
-    iDestruct "Hbody" as (m) "(>Ha & Hblks)".
+    iDestruct "Hbody" as (m) "(>Ha & Hblks & >Hreg)".
     pose proof (ireg_bi_lt inum nib Hin) as Hbi.
     iDestruct (ireg_blks_acc_upd γi γfs inodestart m nib (ireg_bi inum) Hbi
                 with "Hblks") as "[Hblk Hback]".
@@ -275,8 +275,8 @@ Section IregLinkNz.
     rewrite -Hdeq in Hrt.
     assert (Hins : <[islot inum := ds !!! islot inum]> ds = ds).
     { apply list_insert_id, list_lookup_lookup_total_lt. lia. }
-    iMod ("Hclose" with "[Ha Hfsb Harm Hla Hep Hslback Hback]") as "_".
-    { iNext. iExists m. iFrame "Ha".
+    iMod ("Hclose" with "[Ha Hreg Hfsb Harm Hla Hep Hslback Hback]") as "_".
+    { iNext. iExists m. iFrame "Ha Hreg".
       iApply ("Hback" $! m with "[%] [Hfsb Harm Hla Hep Hslback]"); [done |].
       iExists ds. iSplitR; [done |]. iSplitR; [done |].
       iSplitL "Hfsb"; [iExact "Hfsb" |].
@@ -312,7 +312,7 @@ Section IregLinkNz.
     assert (Hkey : (16 * Z.of_nat (ireg_bi inum) + Z.of_nat (islot inum))%Z
                    = bv_unsigned inum) by (symmetry; apply ireg_key_split).
     iMod (inv_acc E iregN with "Hinv") as "[Hbody Hclose]"; [exact HE |].
-    iDestruct "Hbody" as (m) "(>Ha & Hblks)".
+    iDestruct "Hbody" as (m) "(>Ha & Hblks & >Hreg)".
     pose proof (ireg_bi_lt inum nib Hin) as Hbi.
     iDestruct (ireg_blks_acc_upd γi γfs inodestart m nib (ireg_bi inum) Hbi
                 with "Hblks") as "[Hblk Hback]".
@@ -336,8 +336,8 @@ Section IregLinkNz.
     rewrite -Hdeq in Hrt.
     assert (Hins : <[islot inum := ds !!! islot inum]> ds = ds).
     { apply list_insert_id, list_lookup_lookup_total_lt. lia. }
-    iMod ("Hclose" with "[Ha Hfsb Harm Hla Hep Hslback Hback]") as "_".
-    { iNext. iExists m. iFrame "Ha".
+    iMod ("Hclose" with "[Ha Hreg Hfsb Harm Hla Hep Hslback Hback]") as "_".
+    { iNext. iExists m. iFrame "Ha Hreg".
       iApply ("Hback" $! m with "[%] [Hfsb Harm Hla Hep Hslback]"); [done |].
       iExists ds. iSplitR; [done |]. iSplitR; [done |].
       iSplitL "Hfsb"; [iExact "Hfsb" |].
